Added ghost method and code for sameElements

Homework6.dfy
@@ -20,7 +20,7 @@ function treeContains<T>(tree:Tree<T>, element:T):bool
 {
 	match tree
     case Leaf => false
-    case Node(leftTree, rightTree, root) => treeContains(leftTree, element) || treeContains(rightTree, element)
+    case Node(leftTree, rightTree, root) => (root == element) || treeContains(leftTree, element) || treeContains(rightTree, element)
 }
 
 function listContains<T>(xs:List<T>, element:T):bool
@@ -30,9 +30,52 @@ function listContains<T>(xs:List<T>, element:T):bool
     case Cons(x, xs') => (x == element) || listContains(xs', element)
 }
 
+//Based on memberOfAppend from 12May20 lecture example
+ghost method memberOfList<T>(xs:List<T>, ys:List<T>, element: T)
+ensures listContains(append(xs,ys), element) == ( listContains(xs, element)  ||  listContains(ys, element) )
+{
+    match xs
+    case Nil => {}
+    case Cons(x,xs') => {
+        // memberOfAppend(e,xs',ys);  // <-- use the inductive hypothesis
+        // Dafny knows post-condition
+        // member(e,append(xs',ys)) == ( member(e,xs')  ||  member(e,ys) )
+        /*assert member(e,append(xs,ys))
+            == member(e,append(Cons(x,xs'),ys))
+            == member(e,Cons(x,append(xs',ys)))
+            == (e==x) || member(e,append(xs',ys))
+            == (e==x) || member(e,xs') || member(e,ys)
+            == member(e, Cons(x,xs'))  || member(e,ys)
+            == member(e, xs)           || member(e,ys)
+            ;*/
+        calc {
+            listContains(append(xs,ys), element);
+            == listContains(append(Cons(x,xs'),ys), element);
+            == listContains(Cons(x,append(xs',ys)), element);
+            == (element == x) || listContains(append(xs',ys), element);
+            == { memberOfList(xs',ys, element); }
+               (element == x) || listContains(xs', element) || listContains(ys, element);
+            == listContains(Cons(x,xs'), element)  || listContains(ys, element);
+            == listContains(xs, element)           || listContains(ys, element);
+        }
+    }
+}
 
 lemma sameElements<T>(tree:Tree<T>, element:T)
 ensures treeContains(tree, element) <==> listContains(flatten(tree), element)
 {
-	
+	match tree
+    case Leaf => {}
+    case Node(leftTree, rightTree, root) => {
+        calc{
+                treeContains(tree, element);
+            == treeContains(Node(leftTree, rightTree, root), element);
+            == (root == element) || treeContains(leftTree, element) || treeContains(rightTree, element);
+            == treeContains(leftTree, element) || listContains(Cons(root, flatten(rightTree)), element);
+            == listContains(flatten(leftTree), element) || listContains(Cons(root, flatten(rightTree)), element);
+            == listContains(append(flatten(leftTree), Cons(root, flatten(rightTree))), element);
+            == listContains(flatten(Node(leftTree, rightTree, root)), element);
+            == listContains(flatten(tree), element);
+        } 
+    }
 }
